execution/theories/Monads.v
@@ -36,14 +36,14 @@ build_monad_laws {
 Class MonadTrans (m : Type -> Type) (mt : Type -> Type) : Type :=
   { lift : forall {t}, mt t -> m t }.
 
-Global Instance option_monad : Monad option :=
+Global Instance Monad_option : Monad option :=
   {| ret _ t := Some t;
      bind _ _ v f := match v with
                  | Some val => f val
                  | None => None
                  end |}.
 
-Global Instance option_monad_laws : MonadLaws option_monad.
+Global Instance MonadLaws_Monad_option : MonadLaws Monad_option.
 Proof.
   constructor.
   - auto.
